

Problem 1

$$\mathcal{L}(y, y') = (y'(x))^2. \quad \frac{\partial \mathcal{L}}{\partial y} = 0. \quad \frac{d}{dx} \frac{\partial \mathcal{L}}{\partial y'} = 2y''$$

$$\frac{\partial \mathcal{L}}{\partial y} - \frac{d}{dx} \frac{\partial \mathcal{L}}{\partial y'} = 0 \Rightarrow 2y'' = 0$$

$$y' = C$$

$$y = Cx + D$$

$$\begin{aligned} C(0) + D &= 0 \Rightarrow C = 1 \\ C + D &= 1 \Rightarrow D = 0 \end{aligned} \quad y(x) = x \quad (\text{straight line in } [0, 1])$$

Problem 2

$$\mathcal{L}(y, y') = y'(x)^2 + 4y(x)^2. \quad \frac{\partial \mathcal{L}}{\partial y} = 8y \quad \frac{d}{dx} \frac{\partial \mathcal{L}}{\partial y'} = 2y''$$

$$\frac{\partial \mathcal{L}}{\partial y} - \frac{d}{dx} \frac{\partial \mathcal{L}}{\partial y'} = 0 \Rightarrow 8y - 2y'' = 0$$

$$4y - y'' = 0$$

Characteristic equation

$$4 - r^2 = 0 \Rightarrow r = \pm 2$$

$$y(x) = C_1 e^{2x} + C_2 e^{-2x}$$

$$y(0) = C_1 + C_2 = 0. \quad C_1 = -C_2$$

$$y(1) = C_1 e^{2x} - C_1 e^{-2x} = 1$$

$$C_1 = \frac{1}{e^{2x} - e^{-2x}}$$

$$y(x) = \frac{1}{e^{2x} - e^{-2x}} e^{2x} + \frac{1}{e^{-2x} - e^{2x}} e^{-2x}$$

Problem 3.

$$\mathcal{L} = \sqrt{1 + y'(x)^2} dx \cdot \frac{\partial \mathcal{L}}{\partial y} = 0$$

$$\frac{\partial \mathcal{L}}{\partial y} - \frac{d}{dx} \frac{\partial \mathcal{L}}{\partial y'} = 0 \Rightarrow \frac{d}{dx} \frac{\partial \mathcal{L}}{\partial y'} = 0 \Rightarrow \frac{\partial \mathcal{L}}{\partial y'} = \text{constant.}$$

let this constant be k . Thus $\frac{\partial \mathcal{L}}{\partial y'} = k$

$$\frac{\partial \mathcal{L}}{\partial y'} = y'(1 + (y')^2)^{-1/2} = k$$

$$y' = k \sqrt{1 + (y')^2}$$

$$(y')^2 = k^2 + k^2 (y')^2$$

$$(y')^2 (1 - k^2) = k^2$$

$$(y')^2 = \frac{k^2}{(1 - k^2)}$$

$$(y') = \frac{\pm k}{\sqrt{1 - k^2}} = \text{constant.} \quad \text{Let } \frac{\pm k}{\sqrt{1 - k^2}} = A$$

$$y = Ax + B$$

$$y(0) = B = 0$$

$$y(1) = A = 1.$$

$$y(x) = x$$

Problem 4.

$$\text{Beltrami identity: } \mathcal{L} - y'(x) \frac{\partial \mathcal{L}}{\partial y'(x)} = C$$

$$(y')^2 - y^2 - y'(2y') = C$$

$$(y')^2 + y^2 - C = 0$$

$$\frac{(y')^2}{-y^2 - C} = 1$$

$$\frac{y'}{\sqrt{-y^2 - C}} = \pm 1$$

$$\frac{y'}{\sqrt{-y^2 - C}} dy = \pm dx$$

$$\arcsin\left(\frac{y}{\sqrt{-C}}\right) = \pm x + D$$

$$y = \sqrt{-C} \sin(x + D)$$

$$y(x) = \sqrt{-C} \sin(x + D)$$

Boundary conditions

$$y(0) = \sqrt{-C} \sin D = 0$$

$$D = n\pi$$

set $n = 0$.

~~set $n = 0$.~~

$$y(\pi/2) = \sqrt{-C} \sin\left(\frac{\pi}{2}\right) = 1$$

$$\sqrt{-C} = 1$$

$$y(x) = \sin x$$

Problem 5.

$$\mathcal{L} = (y')^2 \quad \text{gives} \quad y'' = 0.$$

$$y' = A, \quad y = Ax + B.$$

$$y(0) = B = 0. \quad \text{If } x=1 \text{ is free, then } \frac{\partial \mathcal{L}}{\partial y'} \eta \Big|_{x=1} = 0$$

$$\frac{\partial \mathcal{L}}{\partial y'} \Big|_{x=1} = 0$$

$$y(x) = 0.$$

$$\begin{aligned} 2y'(1) &= 0 \\ A &= 0 \end{aligned}$$

Interpretation: What curve starting from $y(0)=0$ has the least amount of change? Answer: $y(x)=0$.

Problem 6.

$$J[y] = \int_0^1 ((y')^2 + \lambda y) dx. \quad \frac{\partial \mathcal{L}}{\partial y} = \lambda, \quad \frac{\partial \mathcal{L}}{\partial y'} = 2y', \quad \frac{d}{dx} \frac{\partial \mathcal{L}}{\partial y'} = 2y''$$

$$\lambda - 2y'' = 0$$

$$y'' = \frac{\lambda}{2}, \quad y = \frac{\lambda}{4}x^2 + Ax + B.$$

$$y(0) = B = 0$$

$$y(1) = \frac{\lambda}{4} + A = 0. \quad \frac{\lambda}{4} = -A$$

$$y(x) = \frac{\lambda}{4}x^2 - \frac{\lambda}{4}x$$

$$\int_0^1 y(x) dx = \left[\frac{\lambda}{12}x^3 - \frac{\lambda}{8}x^2 \right] \Big|_0^1 = m$$

$$\frac{\lambda}{12} - \frac{\lambda}{8} = m = \frac{1}{6}.$$

$$\frac{\lambda}{12} - \frac{\lambda}{8} = \frac{2\lambda - 3\lambda}{24} = -\frac{\lambda}{24} = \frac{1}{6}$$

$$\lambda = -4.$$

$$y(x) = x - x^2.$$